A first version of the block verifier with support for ghost instructions?

case_study/RiscvPmp/BlockVer/Verifier.v
@@ -136,11 +136,11 @@ Module BlockVerificationDerived2.
         @exec_block_addr b' _ (term_binop bop.bvadd (persist__term ainstr (ω1 ∘ ω2)) (term_val ty_word bv_instrsize)) apc'
       end.
 
-  Definition exec_double_addr {Σ : World}
-    (req : Assertion (Σ ▻ ("a":: ty_xlenbits))) (b : list AST) : M (STerm ty_xlenbits) Σ :=
-    ω1 ∣ an <- @demonic _ _ ;;
-    ω2 ∣ _ <- produce (w := wsnoc _ _) req (acc_snoc_left ω1 _ an);;
-    @exec_block_addr b _ (persist__term an ω2) (persist__term an ω2).
+  (* Definition exec_double_addr {Σ : World} *)
+  (*   (req : Assertion (Σ ▻ ("a":: ty_xlenbits))) (b : list AST) : M (STerm ty_xlenbits) Σ := *)
+  (*   ω1 ∣ an <- @demonic _ _ ;; *)
+  (*   ω2 ∣ _ <- produce (w := wsnoc _ _) req (acc_snoc_left ω1 _ an);; *)
+  (*   @exec_block_addr b _ (persist__term an ω2) (persist__term an ω2). *)
 
   Definition exec_triple_addr {Σ : World}
     (req : Assertion (Σ ▻ ("a"::ty_xlenbits))) (b : list AST)
@@ -175,6 +175,57 @@ Module BlockVerificationDerived2.
 
 End BlockVerificationDerived2.
 
+Module BlockVerification3.
+
+  Import RiscvPmpBlockVerifSpec.
+  Import RiscvPmpBlockVerifExecutor.
+  Import Symbolic.
+
+  Import ModalNotations.
+  Import BlockVerificationDerived2.
+
+  Inductive AnnotInstr :=
+  | AnnotAST : forall (i : AST), AnnotInstr
+  | AnnotLemmaInvocation : forall (l : 𝑳 [ctx]), AnnotInstr
+  .
+
+  Fixpoint exec_block_addr (b : list AnnotInstr) : ⊢ STerm ty_xlenbits -> STerm ty_xlenbits -> M (STerm ty_xlenbits) :=
+    fun _ ainstr apc =>
+      match b with
+      | nil       => pure apc
+      | cons instr b' =>
+          match instr with
+          | AnnotAST i => ω1 ∣ _ <- assert (formula_relop bop.eq ainstr apc) ;;
+                         ω2 ∣ apc' <- exec_instruction_any i (persist__term apc ω1) ;;
+                         @exec_block_addr b' _ (term_binop bop.bvadd (persist__term ainstr (ω1 ∘ ω2)) (term_val ty_word bv_instrsize)) apc'
+          | AnnotLemmaInvocation l =>
+              ω ∣ _ <- SHeapSpecM.call_lemma (LEnv l) [env];;
+              @exec_block_addr b' _ (persist__term ainstr ω) (persist__term apc ω)
+          end
+      end.
+
+  Definition exec_triple_addr {Σ : World}
+    (req : Assertion (Σ ▻ ("a"::ty_xlenbits))) (b : list AnnotInstr)
+    (ens : Assertion (Σ ▻ ("a"::ty_xlenbits) ▻ ("an"::ty_xlenbits))) : M Unit Σ :=
+    ω1 ∣ a <- @demonic _ _ ;;
+    ω2 ∣ _ <- produce (w := wsnoc _ _) req (acc_snoc_left ω1 _ a) ;;
+    ω3 ∣ na <- @exec_block_addr b _ (persist__term a ω2) (persist__term a ω2) ;;
+    consume (w := wsnoc (wsnoc _ ("a"::ty_xlenbits)) ("an"::ty_xlenbits)) ens
+      (acc_snoc_left (acc_snoc_left (ω1 ∘ ω2 ∘ ω3) _ (persist__term a (ω2 ∘ ω3))) ("an"::ty_xlenbits) na).
+
+  (* This is a VC for triples, for doubles we probably need to talk *)
+  (*    about the continuation of a block. *)
+  Definition VC__addr {Σ : LCtx} (req : Assertion {| wctx := Σ ▻ ("a":: ty_xlenbits); wco := []%ctx |}) (b : list AnnotInstr)
+    (ens : Assertion {| wctx := Σ ▻ ("a"::ty_xlenbits) ▻ ("an"::ty_xlenbits); wco := []%ctx |}) : 𝕊 ε :=
+    SymProp.demonic_close
+      (@exec_triple_addr
+         {| wctx := Σ; wco := []%ctx |}
+         req b ens
+         (* Could include leakcheck here *)
+         (fun _ _ _ _ h => SymProp.block)
+         []%env []%list).
+End BlockVerification3.
+
 Module BlockVerificationDerived2Sound.
   Import RiscvPmpBlockVerifSpec.
   Import RiscvPmpBlockVerifShalExecutor.
@@ -195,7 +246,7 @@ Module BlockVerificationDerived2Sound.
   Definition produce {Σ} : Valuation Σ -> Assertion Σ -> M unit := CHeapSpecM.produce.
   Definition consume {Σ} : Valuation Σ -> Assertion Σ -> M unit := CHeapSpecM.consume.
 
-  Local Notation "x <- ma ;; mb" :=
+  Notation "x <- ma ;; mb" :=
     (bind ma (fun x => mb))
       (at level 80, ma at level 90, mb at level 200, right associativity).
 
@@ -357,6 +408,113 @@ Module BlockVerificationDerived2Sound.
 
 End BlockVerificationDerived2Sound.
 
+Module BlockVerification3Sound.
+  Import RiscvPmpBlockVerifSpec.
+  Import RiscvPmpBlockVerifShalExecutor.
+  Import RiscvPmpIrisInstanceWithContracts.
+  Import BlockVerificationDerived2.
+  Import BlockVerification3.
+  Import BlockVerificationDerived2Sound.
+
+  Fixpoint exec_block_addr__c (b : list AnnotInstr) : Val ty_xlenbits -> Val ty_xlenbits -> M (Val ty_xlenbits) :=
+    fun ainstr apc =>
+      match b with
+      | nil       => pure apc
+      | cons instr b' =>
+          match instr with
+          | AnnotAST i => _ <- assert (ainstr = apc) ;;
+                         apc' <- exec_instruction_any__c i apc ;;
+                         @exec_block_addr__c b' (bv.add ainstr bv_instrsize) apc'
+          | AnnotLemmaInvocation l => 
+              _ <- CHeapSpecM.call_lemma (LEnv l) [env];;
+              exec_block_addr__c b' ainstr apc
+          end
+      end.
+
+  Import refinement.notations.
+
+  Lemma refine_exec_block_addr (b : list AnnotInstr) :
+    ℛ⟦RVal ty_xlenbits -> RVal ty_xlenbits -> RHeapSpecM [ctx] [ctx] (RVal ty_xlenbits)⟧
+      (@BlockVerification3.exec_block_addr b)
+      (exec_block_addr__c b).
+  Proof.
+    induction b as [|instr b].
+    - intros w0 ι0 Hpc0 a ? ->.
+      now apply refine_pure.
+    - intros w0 ι0 Hpc0 ainstr ? -> apc ? ->.
+      destruct instr.
+      + apply refine_bind.
+        apply refine_assert_formula; easy.
+        intros w1 ω1 ι1 -> Hpc1 _ _ _.
+        apply refine_bind.
+        apply refine_exec_instruction_any; auto.
+        eapply refine_inst_persist; eauto; easy.
+        intros w2 ω2 ι2 -> Hpc2 napc ? ->.
+        apply IHb; auto.
+        { cbn. f_equal.
+          change (inst_term ?t ?ι) with (inst t ι).
+          rewrite (inst_persist (H := inst_term) (acc_trans ω1 ω2) _ ainstr).
+          now rewrite ?sub_acc_trans, ?inst_subst.
+        }
+        { reflexivity. }
+      + apply refine_bind.
+        apply refine_call_lemma; easy.
+        intros w ω ι -> Hpc _ _ _.
+        apply IHb; auto; cbn.
+        { now rewrite (inst_persist (H := inst_term) _ _ ainstr). }
+        { now rewrite (inst_persist (H := inst_term) _ _ apc). }
+  Qed.
+
+  Definition exec_triple_addr__c {Σ : World} (ι : Valuation Σ)
+    (req : Assertion (Σ ▻ ("a"::ty_xlenbits))) (b : list AnnotInstr)
+    (ens : Assertion (Σ ▻ ("a"::ty_xlenbits) ▻ ("an"::ty_xlenbits))) : M unit :=
+    a <- @demonic _ ;;
+    _ <- produce (ι ► ( _ ↦ a )) req ;;
+    na <- @exec_block_addr__c b a a ;;
+    consume (ι ► ( ("a"::ty_xlenbits) ↦ a ) ► ( ("an"::ty_xlenbits) ↦ na )) ens.
+
+  Import ModalNotations.
+
+  Lemma refine_exec_triple_addr {Σ : World}
+    (req : Assertion (Σ ▻ ("a"::ty_xlenbits))) (b : list AnnotInstr)
+    (ens : Assertion (Σ ▻ ("a"::ty_xlenbits) ▻ ("an"::ty_xlenbits))) :
+    forall {ι0 : Valuation Σ} (Hpc0 : instprop (wco Σ) ι0),
+      ℛ⟦RHeapSpecM [ctx] [ctx] RUnit⟧@{ι0}
+        (@BlockVerification3.exec_triple_addr Σ req b ens)
+        (exec_triple_addr__c ι0 req b ens).
+  Proof.
+    intros ι0 Hpc0.
+    unfold BlockVerificationDerived2.exec_triple_addr, exec_triple_addr__c.
+    apply refine_bind.
+    { apply refine_demonic; auto. }
+    intros w1 ω1 ι1 -> Hpc1 a ? ->.
+    apply refine_bind.
+    { apply refine_produce; auto.
+      cbn.
+      now rewrite instprop_subst, inst_sub_wk1.
+    }
+    intros w2 ω2 ι2 -> Hpc2 [] [] _.
+    apply refine_bind.
+    { apply refine_exec_block_addr; auto;
+        eapply refine_inst_persist; eauto.
+    }
+    intros w3 ω3 ι3 -> Hpc3 na ? ->.
+    apply refine_consume; auto.
+    cbn -[sub_wk1].
+    now rewrite ?instprop_subst, ?inst_sub_wk1.
+    cbn [acc_snoc_left sub_acc].
+    refine (eq_trans _ (eq_sym (inst_sub_snoc ι3 (sub_snoc (sub_acc (ω1 ∘ ω2 ∘ ω3)) ("a"∷ty_word) (persist__term a (ω2 ∘ ω3))) ("an"::ty_word) na))).
+    f_equal.
+    rewrite inst_sub_snoc.
+    rewrite <-?inst_subst.
+    rewrite H, ?sub_acc_trans.
+    repeat f_equal.
+    change (persist__term a (ω2 ∘ ω3)) with (persist a (ω2 ∘ ω3)).
+    now rewrite (inst_persist (ω2 ∘ ω3) ι3 a), sub_acc_trans, inst_subst.
+  Qed.
+
+End BlockVerification3Sound.
+
 Module BlockVerificationDerived2Sem.
   Import RiscvPmpBlockVerifSpec.
   Import weakestpre.
@@ -378,6 +536,7 @@ Module BlockVerificationDerived2Sem.
       (fun ret _ => (∃ an, lptsreg nextpc an ∗ lptsreg pc an ∗ POST an) ∗ interp_ptsto_instr a instr)%I.
 
   Lemma mono_exec_instruction_any__c {i a} : Monotonic' (exec_instruction_any__c i a).
+  Proof.
     cbv [Monotonic' exec_instruction_any__c bind CHeapSpecM.bind produce_chunk CHeapSpecM.produce_chunk demonic CHeapSpecM.demonic angelic CHeapSpecM.angelic pure CHeapSpecM.pure].
     intros δ P Q PQ h eP v.
     destruct (env.view δ).
@@ -443,8 +602,8 @@ Module BlockVerificationDerived2Sem.
     }
   Qed.
 
-  Local Notation "a '↦' t" := (reg_pointsTo a t) (at level 79).
-  Local Notation "a '↦ₘ' t" := (interp_ptsto a t) (at level 79).
+  Notation "a '↦' t" := (reg_pointsTo a t) (at level 79).
+  Notation "a '↦ₘ' t" := (interp_ptsto a t) (at level 79).
 
   Fixpoint ptsto_instrs `{sailGS Σ} (a : Val ty_word) (instrs : list AST) : iProp Σ :=
     match instrs with
@@ -595,3 +754,206 @@ Module BlockVerificationDerived2Sem.
   Qed.
 
 End BlockVerificationDerived2Sem.
+
+Module BlockVerification3Sem.
+  Import RiscvPmpBlockVerifSpec.
+  Import weakestpre.
+  Import tactics.
+  Import BlockVerificationDerived2.
+  Import Shallow.Executor.
+  Import ctx.resolution.
+  Import ctx.notations.
+  Import env.notations.
+  Import RiscvPmpIrisBase.
+  Import RiscvPmpIrisInstance.
+  Import RiscvPmpIrisInstanceWithContracts.
+  Import RiscvPmpBlockVerifShalExecutor.
+  Import BlockVerificationDerived2Sound.
+  Import BlockVerificationDerived2Sem.
+  Import BlockVerification3.
+  Import BlockVerification3Sound.
+
+  Lemma mono_exec_block_addr {instrs ainstr apc} : Monotonic' (exec_block_addr__c instrs ainstr apc).
+  Proof.
+    revert ainstr apc.
+    induction instrs as [|instr instrs]; cbn.
+    - intros ainstr apc δ P Q PQ h.
+      cbv [pure CHeapSpecM.pure].
+      apply PQ.
+    - destruct instr.
+      + intros ainstr apc.
+        cbv [Monotonic' bind CHeapSpecM.bind assert CHeapSpecM.assert_formula CHeapSpecM.lift_purem CPureSpecM.assert_formula].
+        intros δ P Q PQ h [<- Hverif].
+        split; [reflexivity|].
+        revert Hverif.
+        apply mono_exec_instruction_any__c.
+        intros res h2.
+        apply IHinstrs.
+        intros res2 h3.
+        now apply PQ.
+      + intros ainstr apc.
+        cbv [Monotonic' bind CHeapSpecM.bind assert CHeapSpecM.assert_formula CHeapSpecM.lift_purem CPureSpecM.assert_formula].
+        intros δ P Q PQ h.
+        apply call_lemma_monotonic.
+        intros res δ1 h2.
+        apply IHinstrs.
+        intros res2 h3.
+        destruct (env.view δ), (env.view δ1).
+        now apply PQ.
+  Qed.
+
+  Definition extract_AST (i : AnnotInstr) : option AST :=
+    match i with
+    | AnnotAST a => Some a
+    | _ => None
+    end.
+
+  Lemma sound_exec_block_addr `{sailGS Σ} {instrs ainstr apc} (h : SCHeap) (POST : Val ty_xlenbits -> CStore [ctx] -> iProp Σ) :
+    LemmaSem ->
+    exec_block_addr__c instrs ainstr apc (fun res => liftP (POST res)) [] h ->
+    ⊢ ((interpret_scheap h ∗ lptsreg pc apc ∗ (∃ v, lptsreg nextpc v) ∗ ptsto_instrs ainstr (omap extract_AST instrs)) -∗
+            (∀ an, lptsreg pc an ∗ (∃ v, lptsreg nextpc v) ∗ ptsto_instrs ainstr (omap extract_AST instrs) ∗ POST an [] -∗ WP_loop) -∗
+            WP_loop)%I.
+  Proof.
+    intros lemSem.
+    revert ainstr apc h POST.
+    induction instrs as [|instr instrs]; cbn; intros ainstr apc h POST.
+    - iIntros (Hverif) "(Hpre & Hpc & Hnpc & _) Hk".
+      iApply "Hk"; iFrame.
+      iSplitR; auto.
+      now iApply Hverif.
+    - destruct instr as [instr|lem].
+      + intros [-> Hverif].
+        assert (⊢ semTripleOneInstrStep (interpret_scheap h) instr
+                  (fun an =>
+                     lptsreg pc an ∗ (∃ v, lptsreg nextpc v) ∗ ptsto_instrs (bv.add apc bv_instrsize) (omap extract_AST instrs) -∗
+                     (∀ an2 : Val ty_word, pc ↦ an2 ∗ (∃ v, lptsreg nextpc v) ∗ ptsto_instrs (bv.add apc bv_instrsize) (omap extract_AST instrs) ∗ POST an2 [env] -∗ WP_loop) -∗
+                       WP_loop) apc) as Hverif2.
+        { apply (sound_exec_instruction_any (fun an δ => (lptsreg pc an : iProp Σ) ∗ (∃ v, lptsreg nextpc v : iProp Σ) ∗ ptsto_instrs (bv.add apc bv_instrsize) (omap extract_AST instrs) -∗ (∀ an2 : Val ty_word, pc ↦ an2 ∗ (∃ v, nextpc ↦ v) ∗ ptsto_instrs (bv.add apc bv_instrsize) (omap extract_AST instrs) ∗ POST an2 [env] -∗ WP_loop) -∗ WP_loop)%I).
+          revert Hverif.
+          apply mono_exec_instruction_any__c.
+          intros an h2.
+          unfold liftP; cbn.
+          iIntros (Hverif) "Hh2 (Hpc & Hnpc & Hinstrs) Hk".
+          iApply (IHinstrs (bv.add apc bv_instrsize)%Z an _ _ Hverif with "[$]").
+          iIntros (an2) "(Hpc & Hinstrs & HPOST)".
+          iApply "Hk"; now iFrame.
+        }
+        iIntros "(Hh & Hpc & Hnpc & Hinstr & Hinstrs) Hk".
+        iApply semWP_seq.
+        iApply semWP_call_inline.
+        iApply (semWP_mono with "[Hh Hnpc Hpc Hinstr]").
+        { iApply ((sound_exec_instruction_any (fun an δ => (lptsreg pc an : iProp Σ) ∗ (∃ v, lptsreg nextpc v : iProp Σ) ∗ ptsto_instrs (bv.add apc bv_instrsize) (omap extract_AST instrs) -∗ (∀ an2 : Val ty_word, pc ↦ an2 ∗ (∃ v, nextpc ↦ v) ∗ ptsto_instrs (bv.add apc bv_instrsize) (omap extract_AST instrs) ∗ POST an2 [env] -∗ WP_loop) -∗ WP_loop)%I) with "[$]").
+          revert Hverif.
+          refine (mono_exec_instruction_any__c (h := h) _ _).
+          intros an h2.
+          unfold liftP; cbn.
+          iIntros (Hverif) "Hh2 (Hpc & Hnpc & Hinstrs) Hk".
+          iApply (IHinstrs (bv.add apc bv_instrsize)%Z an _ _ Hverif with "[$]").
+          iIntros (an2) "(Hpc & Hinstrs & HPOST)".
+          iApply "Hk"; now iFrame.
+        }
+        iIntros (_ _) "([%an (Hnpc & Hpc & Hk2)] & Hinstr)".
+        iApply (semWP_call_inline loop).
+        iApply ("Hk2" with "[$Hpc Hnpc $Hinstrs]"); first by iExists _.
+        iIntros (an2) "(Hpc & Hnpc & Hinstrs & HPOST)".
+        iApply ("Hk" with "[$]").
+      + iIntros (Hlemcall) "(Hh & Hpc & Hnpc & Hinstrs) Hk".
+        unfold bind, CHeapSpecM.bind in Hlemcall; cbn.
+        assert (CHeapSpecM.call_lemma (LEnv lem) [env] (fun _ => liftP (fun δ => lptsreg pc apc ∗ (∃ v : Val ty_xlenbits, lptsreg nextpc v) ∗ ptsto_instrs ainstr (omap extract_AST instrs) -∗
+                   (∀ an : Val ty_xlenbits, lptsreg pc an ∗ (∃ v : Val ty_xlenbits, lptsreg nextpc v) ∗ ptsto_instrs ainstr (omap extract_AST instrs) ∗ POST an [env] -∗ WP_loop) -∗ WP_loop)%I) [env] h) as Hcalllemma.
+        { revert Hlemcall.
+          apply call_lemma_monotonic.
+          intros _ δ h2.
+          destruct (env.view δ).
+          unfold liftP; cbn.
+          iIntros (Heb) "Hh2 (Hpc & Hnpc & Hinstrs) Hk".
+          iApply (IHinstrs _ _ _ _ Heb with "[$Hh2 $Hpc $Hnpc $Hinstrs]").
+          now iApply "Hk".
+        }
+        pose proof (Hlem := lemSem _ lem).
+        destruct (call_lemma_sound [env] [env] h _ _ Hcalllemma).
+        cbn in *.
+        iPoseProof (H0 with "Hh") as "(%ι & _ & Hreq & Hk2)".
+        iApply ("Hk2" with "[Hreq] [$Hpc $Hnpc $Hinstrs] Hk").
+        now iApply Hlem.
+  Qed.
+
+  Definition semTripleBlock `{sailGS Σ} (PRE : Val ty_word -> iProp Σ) (instrs : list AnnotInstr) (POST : Val ty_word -> Val ty_word -> iProp Σ) : iProp Σ :=
+    (∀ a,
+    (PRE a ∗ pc ↦ a ∗ (∃ v, nextpc ↦ v) ∗ ptsto_instrs a (omap extract_AST instrs)) -∗
+      (∀ an, pc ↦ an ∗ (∃ v, nextpc ↦ v) ∗ ptsto_instrs a (omap extract_AST instrs) ∗ POST a an -∗ WP_loop) -∗
+      WP_loop)%I.
+  Global Arguments semTripleBlock {Σ} {_} PRE%I instrs POST%I.
+
+  Lemma sound_exec_triple_addr__c `{sailGS Σ} {W : World} {pre post instrs} {ι : Valuation W} :
+    LemmaSem ->
+      (exec_triple_addr__c ι pre instrs post (λ _ _ _ , True) [env] []%list) ->
+    ⊢ semTripleBlock (λ a : Val ty_word, asn.interpret pre (ι.[("a"::ty_xlenbits) ↦ a])) instrs
+      (λ a na : Val ty_word, asn.interpret post (ι.[("a"::ty_xlenbits) ↦ a].[("an"::ty_xlenbits) ↦ na])).
+  Proof.
+    intros lemSem Hexec.
+    iIntros (a) "(Hpre & Hpc & Hnpc & Hinstrs) Hk".
+    specialize (Hexec a).
+    unfold bind, CHeapSpecM.bind, produce in Hexec.
+    assert (interpret_scheap []%list ∗ asn.interpret pre ι.[("a"::ty_word) ↦ a] ⊢
+    (True ∗ lptsreg pc a ∗ (∃ v, lptsreg nextpc v) ∗ ptsto_instrs a (omap extract_AST instrs)) -∗
+      (∀ an, lptsreg pc an ∗ (∃ v, lptsreg nextpc v) ∗ ptsto_instrs a (omap extract_AST instrs) ∗ asn.interpret post (ι.[("a"::ty_xlenbits) ↦ a].[("an"::ty_xlenbits) ↦ an]) -∗ WP_loop) -∗
+      WP_loop)%I as Hverif.
+    { refine (@produce_sound _ _ _ _ (ι.[("a"::ty_word) ↦ a]) pre (fun _ =>
+    (True ∗ lptsreg pc a ∗ (∃ v, lptsreg nextpc v) ∗ ptsto_instrs a (omap extract_AST instrs)) -∗
+      (∀ an, lptsreg pc an ∗ (∃ v, lptsreg nextpc v) ∗ ptsto_instrs a (omap extract_AST instrs) ∗ asn.interpret post (ι.[("a"::ty_xlenbits) ↦ a].[("an"::ty_xlenbits) ↦ an]) -∗ WP_loop) -∗
+      WP_loop)%I [env] []%list _).
+      revert Hexec.
+      apply produce_monotonic.
+      unfold consume.
+      intros _ h Hexec.
+      cbn.
+      assert (
+          ⊢ ((interpret_scheap h ∗ lptsreg pc a ∗ (∃ v, lptsreg nextpc v) ∗ ptsto_instrs a (omap extract_AST instrs)) -∗
+               (∀ an, lptsreg pc an ∗ (∃ v, lptsreg nextpc v) ∗ ptsto_instrs a (omap extract_AST instrs) ∗
+                        asn.interpret post ι.["a"∷ty_word ↦ a].["an"∷ty_word ↦ an]
+                         -∗ WP_loop) -∗
+               WP_loop)%I) as Hverifblock.
+      { apply (sound_exec_block_addr h
+                  (fun an δ => asn.interpret post ι.["a"∷ty_word ↦ a].["an"∷ty_word ↦ an])%I); first easy.
+        refine (mono_exec_block_addr _ _ _ _ _ Hexec).
+        intros res h2 Hcons. cbn.
+        rewrite <-(bi.sep_True (asn.interpret post ι.["a"∷ty_word ↦ a].["an"∷ty_word ↦ res] : iProp Σ)).
+        eapply (consume_sound (fun _ => True%I : iProp Σ)).
+        revert Hcons.
+        refine (consume_monotonic _ _ _ _ _).
+        cbn. now iIntros.
+      }
+      iIntros "Hh".
+      clear -Hverifblock.
+      iIntros "(_ & Hpc & Hnpc & Hinstrs) Hk".
+      iApply (Hverifblock with "[Hh Hpc Hnpc Hinstrs] Hk").
+      iFrame.
+    }
+    iApply (Hverif with "[Hpre] [Hpc Hnpc Hinstrs]");
+      cbn; iFrame.
+  Qed.
+
+  Lemma sound_VC__addr `{sailGS Σ} {Γ} {pre post instrs} :
+    LemmaSem ->
+    safeE (postprocess (BlockVerification3.VC__addr (Σ := Γ) pre instrs post)) ->
+    forall ι,
+    ⊢ semTripleBlock (fun a => asn.interpret pre (ι.[("a"::ty_xlenbits) ↦ a]))
+      instrs
+      (fun a na => asn.interpret post (ι.[("a"::ty_xlenbits) ↦ a].[("an"::ty_xlenbits) ↦ na])).
+  Proof.
+    intros lemSem Hverif ι.
+    apply (sound_exec_triple_addr__c (W := {| wctx := Γ ; wco := []%ctx |}) (pre := pre) (post := post) (instrs := instrs)); first easy.
+    eapply (refine_exec_triple_addr (Σ := {| wctx := Γ ; wco := []%ctx |}) I (ta := λ w1 _ _ _ _, SymProp.block)).
+    all: cycle 3.
+    - rewrite SymProp.wsafe_safe SymProp.safe_debug_safe.
+      apply (safeE_safe env.nil), postprocess_sound in Hverif.
+      rewrite SymProp.safe_demonic_close in Hverif.
+      now apply Hverif.
+    - cbn. now intros.
+    - reflexivity.
+    - reflexivity.
+  Qed.
+
+End BlockVerification3Sem.
